proof/invariants/freeSlot.v
@@ -102,7 +102,7 @@ nullAddrExists s
 /\ nbPrepareIsNbKern s
 /\ pdchildIsPDT s
 /\ childBlockNullIfChildNull s
-(*/\ childLocHasSameStart s*).
+/\ accessibleBlocksArePresent s.
 
 
 Lemma freeSlot (pd blockToFree: paddr) (P : state -> Prop) :
@@ -4341,7 +4341,7 @@ split.
   (* END pdchildIsPDT *)
 }
 
-(*split.*)
+split.
 { (* BEGIN childBlockNullIfChildNull s *)
   assert(Hcons0: childBlockNullIfChildNull s0) by (unfold cons1Free in *; intuition).
   intros part block sh1entryaddr HpartBisIsPart HblockMapped Hsh1 HPDchild.
@@ -4405,97 +4405,29 @@ split.
   specialize(Hcons0 part block sh1entryaddr HpartBisIsPart HblockMappeds0 Hsh1 HPDchild).
   unfold sh1entryInChildLocation in *. destruct (lookup sh1entryaddr (memory s0) beqAddr); try(congruence).
   destruct v; try(congruence). destruct Hcons0 as (Hcons0 & _). split; trivial. intro. exfalso; congruence.
-  (* END pdchildIsPDT *)
+  (* END childBlockNullIfChildNull *)
 }
 
-(*{ (* BEGIN childLocHasSameStart s *)
-  assert(Hcons0: childLocHasSameStart s0) by (unfold cons1Free in *; intuition).
-  intros part block sh1entryaddr blockChild idchild HpartIsPart HblockMapped Hsh1 HPDchild Hloc HbeqIdChildNull
-    HbeqBCNull startaddr Hstart. rewrite HgetPartsEqs in *. assert(isPDT part s2).
-  { rewrite <-HgetPartsEqs2 in *. apply partitionsArePDT; trivial. }
-  assert(HblockMappeds0: In block (getMappedBlocks part s0)).
-  {
-    destruct (beqAddr pd part) eqn:HbeqParts.
-    - rewrite <-DTL.beqAddrTrue in HbeqParts. subst part. specialize(HgetMappedBPdss0 block).
-      destruct HgetMappedBPdss0 as (_ & Hres & _). apply Hres; assumption.
-    - rewrite <-beqAddrFalse in *. rewrite <-HgetMappedBEqss0; assumption.
-  }
-  assert(HPflag: bentryPFlag block true s).
-  {
-    apply mappedBlockIsBE in HblockMapped. destruct HblockMapped as [bentry (Hlookup & Hpres)]. unfold bentryPFlag.
-    rewrite Hlookup. auto.
-  }
-  unfold sh1entryAddr in *. unfold bentryStartAddr in *. unfold bentryPFlag in *. rewrite Hs in Hstart.
-  rewrite Hs6 in Hstart. rewrite Hs in Hsh1. rewrite Hs6 in Hsh1. rewrite Hs in HPflag. rewrite Hs6 in HPflag.
-  simpl in *. destruct (beqAddr pd block) eqn:HbeqPartBlockBis; try(exfalso; congruence). rewrite beqAddrTrue in *.
+{ (* BEGIN accessibleBlocksArePresent s *)
+  assert(Hcons0: accessibleBlocksArePresent s0) by (unfold cons1Free in *; intuition). intros block HAflag.
+  unfold bentryAFlag in *. unfold bentryPFlag. rewrite Hs. rewrite Hs in HAflag. rewrite Hs6. rewrite Hs6 in HAflag.
+  simpl in *. rewrite beqAddrTrue in *. destruct (beqAddr pd block) eqn:HbeqPartBlockB; try(congruence).
   rewrite <-beqAddrFalse in *. rewrite removeDupIdentity in *; try(apply not_eq_sym); trivial.
-  rewrite removeDupIdentity in *; try(apply not_eq_sym); trivial. rewrite Hs5 in Hstart. rewrite Hs5 in Hsh1.
-  rewrite Hs5 in HPflag. simpl in *. destruct (beqAddr blockToFree block) eqn:HbeqBlocks.
-  { rewrite HnewB2 in HPflag. simpl in *. rewrite HnewB in HPflag. simpl in *. exfalso; congruence. }
-  rewrite <-beqAddrFalse in *. rewrite removeDupIdentity in *; try(apply not_eq_sym); trivial. rewrite Hs4 in Hstart.
-  rewrite Hs4 in Hsh1. simpl in *.
+  rewrite removeDupIdentity in *; try(apply not_eq_sym); trivial. rewrite Hs5 in HAflag. rewrite Hs5.
+  simpl in *. destruct (beqAddr blockToFree block) eqn:HbeqBlocks.
+  { rewrite HnewB2 in HAflag. simpl in *. rewrite HnewB in HAflag. simpl in *. exfalso; congruence. }
+  rewrite <-beqAddrFalse in *. rewrite removeDupIdentity in *; try(apply not_eq_sym); trivial. rewrite Hs4 in HAflag.
+  rewrite Hs4. simpl in *.
   destruct (beqAddr (CPaddr (blockToFree + scoffset)) block) eqn:HbeqSceBlockBis; try(exfalso; congruence).
-  rewrite <-beqAddrFalse in *. rewrite removeDupIdentity in *; try(apply not_eq_sym); trivial. rewrite Hs3 in Hstart.
-  rewrite Hs3 in Hsh1. simpl in *.
+  rewrite <-beqAddrFalse in *. rewrite removeDupIdentity in *; try(apply not_eq_sym); trivial. rewrite Hs3 in HAflag.
+  rewrite Hs3. simpl in *.
   destruct (beqAddr (CPaddr (blockToFree + sh1offset)) block) eqn:HbeqSh1BlockBis; try(exfalso; congruence).
-  rewrite <-beqAddrFalse in *. rewrite removeDupIdentity in *; try(apply not_eq_sym); trivial. rewrite Hs2 in Hstart.
-  rewrite Hs2 in Hsh1. simpl in *. rewrite beqAddrFalse in *. rewrite HbeqBlocks in *.
-  rewrite <-beqAddrFalse in *. rewrite removeDupIdentity in *; try(apply not_eq_sym); trivial. rewrite Hs1 in Hstart.
-  rewrite Hs1 in Hsh1. simpl in *. rewrite beqAddrFalse in *.
-  rewrite HbeqPartBlockBis in *. rewrite <-beqAddrFalse in *.
-  rewrite removeDupIdentity in *; try(apply not_eq_sym); trivial. unfold sh1entryPDchild in *. rewrite Hs in HPDchild.
-  unfold sh1entryInChildLocationWeak in *. rewrite Hs6 in HPDchild. rewrite Hs in Hloc. rewrite Hs6 in Hloc.
-  simpl in *. destruct (beqAddr pd sh1entryaddr) eqn:HbeqPartSh1Bis; try(exfalso; congruence).
-  rewrite beqAddrTrue in *.
-  rewrite <-beqAddrFalse in *. rewrite removeDupIdentity in *; try(apply not_eq_sym); trivial.
-  rewrite removeDupIdentity in *; try(apply not_eq_sym); trivial. rewrite Hs5 in HPDchild. rewrite Hs5 in Hloc.
-  simpl in *. destruct (beqAddr blockToFree sh1entryaddr) eqn:HbeqBlockSh1Bis; try(exfalso; congruence).
-  rewrite <-beqAddrFalse in *. rewrite removeDupIdentity in *; try(apply not_eq_sym); trivial.
-  rewrite Hs4 in HPDchild. rewrite Hs4 in Hloc. simpl in *.
-  destruct (beqAddr (CPaddr (blockToFree + scoffset)) sh1entryaddr) eqn:HbeqSceSh1Bis; try(exfalso; congruence).
-  rewrite <-beqAddrFalse in *. rewrite removeDupIdentity in *; try(apply not_eq_sym); trivial.
-  rewrite Hs3 in HPDchild. rewrite Hs3 in Hloc. simpl in *.
-  destruct (beqAddr (CPaddr (blockToFree + sh1offset)) sh1entryaddr) eqn:HbeqSh1s.
-  {
-    rewrite <-DTL.beqAddrTrue in HbeqSh1s. subst sh1entryaddr. exfalso.
-    destruct (lookup block (memory s0) beqAddr); try(congruence). destruct v; try(congruence).
-    apply CPaddrAddEq in Hsh1; trivial. congruence.
-  }
-  rewrite <-beqAddrFalse in *. rewrite removeDupIdentity in *; try(apply not_eq_sym); trivial.
-  rewrite Hs2 in HPDchild. rewrite Hs2 in Hloc. simpl in *. rewrite beqAddrFalse in *.
-  rewrite HbeqBlockSh1Bis in *. rewrite <-beqAddrFalse in *.
-  rewrite removeDupIdentity in *; try(apply not_eq_sym); trivial. rewrite Hs1 in HPDchild. rewrite Hs1 in Hloc.
-  simpl in *. rewrite beqAddrFalse in *. rewrite HbeqPartSh1Bis in *. rewrite <-beqAddrFalse in *.
-  rewrite removeDupIdentity in *; try(apply not_eq_sym); trivial.
-  specialize(Hcons0 part block sh1entryaddr blockChild idchild HpartIsPart HblockMappeds0 Hsh1 HPDchild Hloc
-    HbeqIdChildNull HbeqBCNull startaddr Hstart). unfold bentryStartAddr in *. rewrite Hs. rewrite Hs6. simpl.
-  destruct (beqAddr pd blockChild) eqn:HbeqPartBC.
-  { rewrite <-DTL.beqAddrTrue in HbeqPartBC. subst blockChild. rewrite HlookupParts0 in *. congruence. }
-  rewrite beqAddrTrue. rewrite <-beqAddrFalse in *.
-  rewrite removeDupIdentity; try(apply not_eq_sym); trivial.
-  rewrite removeDupIdentity; try(apply not_eq_sym); trivial. rewrite Hs5. simpl. (*Nope*)
-  destruct (beqAddr blockToFree blockChild) eqn:HbeqBlockBC.
-  { rewrite <-DTL.beqAddrTrue in HbeqBlockBC. subst blockChild. rewrite HlookupBlockToF in *. congruence. }
-  rewrite <-beqAddrFalse in *. rewrite removeDupIdentity; try(apply not_eq_sym); trivial. rewrite Hs4. simpl.
-  destruct (beqAddr (CPaddr (blockToFree + scoffset)) blockChild) eqn:HbeqSceBC.
-  {
-    rewrite <-DTL.beqAddrTrue in HbeqSceBC. rewrite HbeqSceBC in *. rewrite Hnone in *. exfalso; congruence.
-  }
-  rewrite <-beqAddrFalse in *. rewrite removeDupIdentity; try(apply not_eq_sym); trivial. rewrite Hs3. simpl.
-  destruct (beqAddr (CPaddr (blockToFree + sh1offset)) blockChild) eqn:HbeqSh1BC.
-  {
-    rewrite <-DTL.beqAddrTrue in HbeqSh1BC. rewrite HbeqSh1BC in *. rewrite Hnone in *. exfalso; congruence.
-  }
-  rewrite <-beqAddrFalse in *. rewrite removeDupIdentity; try(apply not_eq_sym); trivial. rewrite Hs2. simpl.
-  rewrite beqAddrFalse in *. rewrite HbeqBlockBC. rewrite <-beqAddrFalse in *.
-  rewrite removeDupIdentity; try(apply not_eq_sym); trivial. rewrite Hs1. simpl. rewrite beqAddrFalse in *.
-  rewrite HbeqPartAddr. rewrite <-beqAddrFalse in *. rewrite removeDupIdentity; try(apply not_eq_sym); trivial.
-  
-  
-  
-  
-  
-  
-  (* END childLocHasSameStart *)
-}*)
+  rewrite <-beqAddrFalse in *. rewrite removeDupIdentity in *; try(apply not_eq_sym); trivial. rewrite Hs2 in HAflag.
+  rewrite Hs2. simpl in *. rewrite beqAddrFalse in *. rewrite HbeqBlocks in *.
+  rewrite <-beqAddrFalse in *. rewrite removeDupIdentity in *; try(apply not_eq_sym); trivial. rewrite Hs1 in HAflag.
+  rewrite Hs1. simpl in *. rewrite beqAddrFalse in *.
+  rewrite HbeqPartBlockB in *. rewrite <-beqAddrFalse in *.
+  rewrite removeDupIdentity in *; try(apply not_eq_sym); trivial. apply Hcons0; trivial.
+  (* END accessibleBlocksArePresent *)
+}
 Qed.
